lemmas of first assignment added

Unification.thy
@@ -11,10 +11,34 @@ fun fv :: "('f, 'v) term \<Rightarrow> 'v set" where
 type_synonym ('f, 'v) subst = "'v \<Rightarrow> ('f, 'v) term"
 
 fun sapply :: "('f, 'v) subst \<Rightarrow> ('f, 'v) term \<Rightarrow> ('f, 'v) term" (infixr "\<cdot>" 67) where 
+  "sapply _ x = x" 
 
 fun scomp :: "('f, 'v) subst \<Rightarrow> ('f, 'v) subst \<Rightarrow> ('f, 'v) subst" (infixl "\<circ>s" 75) where
 
 lemma fv_sapply: "fv (\<sigma> \<cdot> t) = (\<Union>x \<in> fv t. fv (\<sigma> x))"
+  sorry
+
+lemma sapply_cong:
+  assumes "\<And>x. x \<in> fv t \<Longrightarrow> \<sigma> x = \<tau> x"
+  shows "\<sigma> \<cdot> t = \<tau> \<cdot> t"
+  sorry
+
+lemma scomp_sapply: "(\<sigma> \<circ>s \<tau>) x = \<sigma> \<cdot> (\<tau> \<cdot> x)"
+  sorry
+
+lemma sapply_scomp_distr: "(\<sigma> \<circ>s \<tau>) \<cdot> t = \<sigma> \<cdot> (\<tau> \<cdot> t)"
+  sorry
+
+lemma scomp_assoc: "(\<sigma> \<circ>s \<tau>) \<circ>s \<rho> = \<sigma> \<circ>s (\<tau> \<circ>s \<rho>)"
+  sorry
+
+lemma scomp_var [simp]: "\<sigma> \<circ>s Var = \<sigma>"
+  sorry
+
+lemma var_scomp [simp]: "Var \<circ>s \<sigma> = \<sigma>"
+  sorry
+
+
 
 
 
